Impl/DeallocModel.i.dfy
@@ -3,6 +3,7 @@ include "BookkeepingModel.i.dfy"
 module DeallocModel { 
   import opened StateModel
   import opened IOModel
+  import opened DiskOpModel
   import opened BookkeepingModel
   import opened Bounds
   import opened ViewOp
