Impl/QueryImpl.i.dfy
@@ -16,6 +16,7 @@ module QueryImpl {
   import opened StateImpl
   import opened BucketImpl
   import opened EvictImpl
+  import opened DiskOpImpl
 
   import opened Options
   import opened NativeTypes
@@ -39,6 +40,7 @@ module QueryImpl {
   requires io.initialized()
   requires Inv(k, s)
   requires io !in s.Repr()
+  requires s.ready
   modifies io
   modifies s.Repr()
   ensures WellUpdated(s)
@@ -47,68 +49,63 @@ module QueryImpl {
     QueryModel.reveal_query();
     QueryModel.reveal_queryIterate();
 
-    if (!s.ready) {
-      PageInIndirectionTableReq(k, s, io);
-      res := None;
-    } else {
-      var ref := BT.G.Root();
-      var msg := ValueMessage.IdentityMessage();
-      var counter: uint64 := 40;
+    var ref := BT.G.Root();
+    var msg := ValueMessage.IdentityMessage();
+    var counter: uint64 := 40;
 
-      // TODO write this in recursive style, it would be a lot simpler?
-      while true
-      invariant Inv(k, s)
-      invariant s.ready
-      invariant ref in SM.IIndirectionTable(IIndirectionTable(s.ephemeralIndirectionTable)).graph
-      invariant io.initialized()
-      invariant forall s', r, io' ::
-          QueryModel.queryIterate(Ic(k), s.I(), key, msg, ref, IIO(io), counter, s', r, io') ==>
-          QueryModel.query(Ic(k), old(s.I()), old(IIO(io)), key, s', r, io')
-      invariant counter as int >= 0
-      invariant io !in s.Repr()
-      invariant WellUpdated(s)
-      decreases counter as int
-      {
-        if counter == 0 {
-          res := None;
-          return;
-        }
+    // TODO write this in recursive style, it would be a lot simpler?
+    while true
+    invariant Inv(k, s)
+    invariant s.ready
+    invariant ref in SM.IIndirectionTable(IIndirectionTable(s.ephemeralIndirectionTable)).graph
+    invariant io.initialized()
+    invariant forall s', r, io' ::
+        QueryModel.queryIterate(Ic(k), s.I(), key, msg, ref, IIO(io), counter, s', r, io') ==>
+        QueryModel.query(Ic(k), old(s.I()), old(IIO(io)), key, s', r, io')
+    invariant counter as int >= 0
+    invariant io !in s.Repr()
+    invariant WellUpdated(s)
+    decreases counter as int
+    {
+      if counter == 0 {
+        res := None;
+        return;
+      }
 
-        var nodeOpt := s.cache.GetOpt(ref);
-        if (nodeOpt.None?) {
-          PageInReqOrMakeRoom(k, s, io, ref);
-          res := None;
+      var nodeOpt := s.cache.GetOpt(ref);
+      if (nodeOpt.None?) {
+        PageInNodeReqOrMakeRoom(k, s, io, ref);
+        res := None;
+        return;
+      } else {
+        var node := nodeOpt.value;
+
+        node.LemmaReprSeqBucketsLeRepr();
+        s.cache.LemmaNodeReprLeRepr(ref);
+        MutBucket.reveal_ReprSeq();
+
+        ghost var oldIVars := s.I();
+        LruModel.LruUse(s.lru.Queue, ref);
+        s.lru.Use(ref);
+        assert SM.IBlockCache(oldIVars) == SM.IBlockCache(s.I());
+
+        var r := Pivots.ComputeRoute(node.pivotTable, key);
+        var bucket := node.buckets[r];
+
+        var kmtMsg := bucket.Query(key);
+        var newmsg := if kmtMsg.Some? then ValueMessage.Merge(msg, kmtMsg.value) else msg;
+
+        if (newmsg.Define?) {
+          res := Some(newmsg.value);
           return;
         } else {
-          var node := nodeOpt.value;
-
-          node.LemmaReprSeqBucketsLeRepr();
-          s.cache.LemmaNodeReprLeRepr(ref);
-          MutBucket.reveal_ReprSeq();
-
-          ghost var oldIVars := s.I();
-          LruModel.LruUse(s.lru.Queue, ref);
-          s.lru.Use(ref);
-          assert SM.IVars(oldIVars) == SM.IVars(s.I());
-
-          var r := Pivots.ComputeRoute(node.pivotTable, key);
-          var bucket := node.buckets[r];
-
-          var kmtMsg := bucket.Query(key);
-          var newmsg := if kmtMsg.Some? then ValueMessage.Merge(msg, kmtMsg.value) else msg;
-
-          if (newmsg.Define?) {
-            res := Some(newmsg.value);
-            return;
+          if node.children.Some? {
+            BookkeepingModel.lemmaChildInGraph(Ic(k), s.I(), ref, node.children.value[r]);
+            counter := counter - 1;
+            ref := node.children.value[r];
           } else {
-            if node.children.Some? {
-              BookkeepingModel.lemmaChildInGraph(Ic(k), s.I(), ref, node.children.value[r]);
-              counter := counter - 1;
-              ref := node.children.value[r];
-            } else {
-              res := Some(ValueType.DefaultValue());
-              return;
-            }
+            res := Some(ValueType.DefaultValue());
+            return;
           }
         }
       }
